Use the fancy environment everywhere

rupicola/stlc/Compiler.fst
@@ -37,7 +37,7 @@ let test2 : compile_typ ((unit -> bool) -> (bool -> unit)) = solve
 let _ = assert (test2.r == QArr (QArr QUnit QBool) (QArr QBool QUnit))
 
 (** Compiling expressions **)
-class compile_exp (#a:Type0) {| ca: compile_typ a |} (g:env) (fs_e:fs_env g -> a) = { (** using fs_oexp g (pack ca) complicates the instances of the type class **)
+class compile_exp (#a:Type0) {| ca: compile_typ a |} (g:typ_env) (fs_e:eval_env g -> a) = { (** using fs_oexp g (pack ca) complicates the instances of the type class **)
   [@@@no_method] e : (e:exp{fv_in_env g e}); (** expression is closed by g *)
 
   (** The following two lemmas are independent one of the other (we don't use one to prove the other). **)
@@ -81,14 +81,14 @@ let test_false : compile_closed false = solve
 
 (** fs_hd' works better with typeclass resolution than fs_hd **)
 [@"opaque_to_smt"] (** not sure if it is the right pragma to prevent F* unfolding get_v' during type class resolution **)
-val fs_hd' : #g:env -> #t:qType -> fs_env (extend t g) -> a:Type{a == get_Type t} -> a
-let fs_hd' #g fsG a =
-  fs_hd #g fsG
+val hd' : #g:typ_env -> #t:qType -> eval_env (extend t g) -> a:Type{a == get_Type t} -> a
+let hd' #g fsG a =
+  hd fsG
 
 instance compile_exp_var
-  (g:env)
+  (g:typ_env)
   (a:Type) {| ca:compile_typ a |}
-  : compile_exp #a #ca (extend (pack ca) g) (fun fsG -> fs_hd' fsG a) = {
+  : compile_exp #a #ca (extend (pack ca) g) (fun fsG -> hd' fsG a) = {
     e = EVar 0;
     equiv_proof = (fun () ->
       admit () (** this needs more refactoring **)
@@ -97,13 +97,13 @@ instance compile_exp_var
    );
 }
 
-let test1_var : compile_exp (extend tunit empty) (fun fsG -> fs_hd' fsG unit) = solve
+let test1_var : compile_exp (extend tunit empty) (fun fsG -> hd' fsG unit) = solve
 
 instance compile_exp_var_shrink1 (** CA: how to make this general? **)
-  (g:env)
+  (g:typ_env)
   (a:Type) {| ca:compile_typ a |}
   (t:qType)
-  : compile_exp (extend t (extend (pack ca) g)) (fun fsG -> fs_hd' (fs_tail fsG) a) = {
+  : compile_exp (extend t (extend (pack ca) g)) (fun fsG -> hd' (tail fsG) a) = {
     e = EVar 1;
     equiv_proof = (fun () -> admit ()
     (**
@@ -116,8 +116,8 @@ instance compile_exp_var_shrink1 (** CA: how to make this general? **)
 instance compile_exp_var_shrink2 (** CA: how to make this general? **)
   (a:Type) {| ca:compile_typ a |}
   (t1 t2:qType)
-  (g:env)
-  : compile_exp (extend t1 (extend t2 (extend (pack ca) g))) (fun fsG -> fs_hd' (fs_tail (fs_tail fsG)) a) = {
+  (g:typ_env)
+  : compile_exp (extend t1 (extend t2 (extend (pack ca) g))) (fun fsG -> hd' (tail (tail fsG)) a) = {
     e = EVar 2;
     equiv_proof = (fun () -> admit ()
       (** This needs more refactoring
@@ -126,18 +126,18 @@ instance compile_exp_var_shrink2 (** CA: how to make this general? **)
       ce.equiv_proof ()); **))
   }
 
-let test2_var : compile_exp (extend tunit (extend tunit empty)) (fun fsG -> fs_hd' (fs_tail fsG) unit) =
+let test2_var : compile_exp (extend tunit (extend tunit empty)) (fun fsG -> hd' (tail fsG) unit) =
   solve
 
-let test3_var : compile_exp (extend tunit (extend tunit (extend tunit empty))) (fun fsG -> fs_hd' (fs_tail (fs_tail fsG)) unit) =
+let test3_var : compile_exp (extend tunit (extend tunit (extend tunit empty))) (fun fsG -> hd' (tail (tail fsG)) unit) =
   solve
 
 instance compile_exp_lambda
   g
   (a:Type) {| ca: compile_typ a |}
   (b:Type) {| cb: compile_typ b |}
-  (f:fs_env g -> a -> b)
-  {| cf: compile_exp #b #cb (extend (pack ca) g) (fun fsG -> f (fs_tail #(pack ca) fsG) (fs_hd' fsG a)) |}
+  (f:eval_env g -> a -> b)
+  {| cf: compile_exp #b #cb (extend (pack ca) g) (fun fsG -> f (tail #(pack ca) fsG) (hd' fsG a)) |}
   : compile_exp g f = {
   e = begin
     lem_fv_in_env_lam g (pack ca) cf.e;
@@ -145,8 +145,8 @@ instance compile_exp_lambda
   end;
   equiv_proof = (fun () ->
     cf.equiv_proof ();
-    reveal_opaque (`%fs_hd') (fs_hd' #g #(pack ca));
-    equiv_lam g (pack ca) cf.e (pack cb) f
+    reveal_opaque (`%hd') (hd' #g #(pack ca));
+    equiv_lam g (pack ca) (pack cb) f cf.e
   )
 }
 
@@ -177,8 +177,8 @@ instance compile_exp_app
   g
   (a:Type) {| ca: compile_typ a |}
   (b:Type) {| cb: compile_typ b |}
-  (f:fs_env g -> a -> b) {| cf: compile_exp #_ #solve g f |}
-  (x:fs_env g -> a)     {| cx: compile_exp #_ #ca g x |}
+  (f:eval_env g -> a -> b) {| cf: compile_exp #_ #solve g f |}
+  (x:eval_env g -> a)     {| cx: compile_exp #_ #ca g x |}
   : compile_exp #_ #cb g (fun fsG -> (f fsG) (x fsG)) = {
   e = begin
     lem_fv_in_env_app g cf.e cx.e;
@@ -187,7 +187,7 @@ instance compile_exp_app
   equiv_proof = (fun () ->
     cf.equiv_proof ();
     cx.equiv_proof ();
-    equiv_app g (pack ca) (pack cb) cf.e cx.e f x
+    equiv_app g (pack ca) (pack cb) f x cf.e cx.e
   );
 }
 
@@ -214,11 +214,11 @@ let _ = assert (test2_topf.e == EApp (ELam (ELam (EVar 1))) EUnit \/
 
 instance compile_exp_if
   g
-  (co:fs_env g -> bool)  {| cco: compile_exp #_ #solve g co |}
+  (co:eval_env g -> bool)  {| cco: compile_exp #_ #solve g co |}
 
   (a:Type) {| ca: compile_typ a |}
-  (th:fs_env g -> a)     {| cth: compile_exp #_ #ca g th |}
-  (el:fs_env g -> a)     {| cel: compile_exp #_ #ca g el |}
+  (th:eval_env g -> a)     {| cth: compile_exp #_ #ca g th |}
+  (el:eval_env g -> a)     {| cel: compile_exp #_ #ca g el |}
   : compile_exp #_ #ca g (fun fsG -> if co fsG then th fsG else el fsG) = {
   e = begin
     lem_fv_in_env_if g cco.e cth.e cel.e;
@@ -228,7 +228,7 @@ instance compile_exp_if
     cco.equiv_proof ();
     cth.equiv_proof ();
     cel.equiv_proof ();
-    equiv_if g (pack ca) cco.e cth.e cel.e co th el
+    equiv_if g (pack ca) co th el cco.e cth.e cel.e
   );
 }
 
@@ -245,7 +245,7 @@ let test1_hoc : compile_closed
   #((bool -> bool) -> bool)
   #(compile_typ_arrow _ _ #(compile_typ_arrow _ _ #compile_typ_bool #compile_typ_bool))
   (fun f -> f false) =
-  compile_exp_lambda _ _ _ _ #(compile_exp_app _ _ _ (fun fsG -> fs_hd' fsG (bool -> bool)) _)
+  compile_exp_lambda _ _ _ _ #(compile_exp_app _ _ _ (fun fsG -> hd' fsG (bool -> bool)) _)
 
 let _ = assert (test1_hoc.e == ELam (EApp (EVar 0) EFalse))
 
@@ -253,8 +253,8 @@ instance compile_exp_pair
   g
   (a:Type) {| ca: compile_typ a |}
   (b:Type) {| cb: compile_typ b |}
-  (l:fs_env g -> a)     {| cl: compile_exp #_ #ca g l |}
-  (r:fs_env g -> b)     {| cr: compile_exp #_ #cb g r |}
+  (l:eval_env g -> a)     {| cl: compile_exp #_ #ca g l |}
+  (r:eval_env g -> b)     {| cr: compile_exp #_ #cb g r |}
   : compile_exp #(a & b) g (fun fsG -> (l fsG, r fsG)) = {
   e = begin
     lem_fv_in_env_pair g cl.e cr.e;
@@ -263,7 +263,7 @@ instance compile_exp_pair
   equiv_proof = (fun () ->
     cl.equiv_proof ();
     cr.equiv_proof ();
-    equiv_pair g (pack ca) (pack cb) cl.e cr.e l r
+    equiv_pair g (pack ca) (pack cb) l r cl.e cr.e
   );
 }
 
@@ -287,7 +287,7 @@ instance compile_exp_pair_fst
   equiv_proof = (fun () ->
     equiv_pair_fst g (pack ca) (pack cb);
     assert (
-      (mk_arrow (mk_pair (pack ca) (pack cb)) (pack ca)) ==
+      (((pack ca) ^* (pack cb)) ^-> (pack ca)) ==
       (pack (compile_typ_arrow (a & b) a #(compile_typ_pair a b #ca #cb) #ca))) by (compute ())
   );
 }
@@ -315,7 +315,7 @@ instance compile_exp_snd
   equiv_proof = (fun () ->
     equiv_pair_snd g (pack ca) (pack cb);
     assert (
-      (mk_arrow (mk_pair (pack ca) (pack cb)) (pack cb)) ==
+      (((pack ca) ^* (pack cb)) ^-> (pack cb)) ==
       (pack (compile_typ_arrow (a & b) b #(compile_typ_pair a b #ca #cb) #cb))) by (compute ())
   );
 }
