rupicola/stlc/ExpRel.fst
@@ -1,40 +1,390 @@
 module ExpRel
 
-open FStar.FunctionalExtensionality
+open FStar.Tactics
+open FStar.Classical.Sugar
+open FStar.List.Tot
 
-type fs_env g =
-  restricted_t (x:var{Some? (g x)}) (fun x -> get_Type (Some?.v (g x)))
+open STLC
+open QTyp
 
-let fs_empty : fs_env empty =
-  on_dom
-    (x:var{Some? (empty x)})
-    #(fun x -> get_Type (Some?.v (empty x)))
-    (fun _ -> assert False)
+(** Cross Language Binary Logical Relation between F* and STLC expressions
+     for __closed terms__. **)
+let rec (∋) (t:qType) (p:get_Type t * closed_exp) : Tot Type0 (decreases %[get_rel t;0]) =
+  let fs_v = fst p in
+  let e = snd p in
+  match get_rel t with // way to "match" on F* types
+  | QUnit -> fs_v == () /\ e == EUnit
+  | QBool -> (fs_v == true /\ e == ETrue) \/ (fs_v == false /\ e == EFalse)
+  | QArr #s1 #s2 r1 r2 -> begin
+    let fs_f : s1 -> s2 = fs_v in
+    match e with
+    | ELam e' ->
+      (forall (v:value) (fs_v:s1). (| s1, r1 |) ∋ (fs_v, v) ==>
+        (| s2, r2 |) ⦂ (fs_f fs_v, subst_beta v e'))
+    | _ -> False
+  end
+  | QPair #s1 #s2 r1 r2 -> begin
+    match e with
+    | EPair e1 e2 ->
+      (| s1, r1 |) ∋ (fst #s1 #s2 fs_v, e1) /\ (| s2, r2 |) ∋ (snd #s1 #s2 fs_v, e2)
+    | _ -> False
+  end
+and (⦂) (t:qType) (p: get_Type t * closed_exp) : Tot Type0 (decreases %[get_rel t;1]) =
+  let fs_e = fst p in
+  let e = snd p in
+  forall (e':closed_exp). steps e e' ==> irred e' ==> t ∋ (fs_e, e')
 
-let fs_stack #g fsG #t fs_v =
-  on_dom
-    (x:var{Some? ((extend t g) x)})
-    #(fun x -> get_Type (Some?.v ((extend t g) x)))
-    (fun y ->
-      if y = 0 then fs_v else fsG (y-1))
+let lem_values_are_expressions t fs_e e : (** lemma used by Amal **)
+  Lemma (requires t ∋ (fs_e, e))
+        (ensures  t ⦂ (fs_e, e)) = admit ()
 
-let fs_hd #g fsG = fsG 0
+let rec lem_values_are_values t fs_e (e:closed_exp) :
+  Lemma (requires t ∋ (fs_e, e))
+        (ensures is_value e)
+        (decreases e) =
+  match get_rel t with
+  | QUnit -> ()
+  | QBool -> ()
+  | QArr #s1 #s2 r1 r2 -> ()
+  | QPair #s1 #s2 r1 r2 ->
+    let EPair e1 e2 = e in
+    lem_values_are_values (| s1, r1 |) (fst #s1 #s2 fs_e) e1;
+    lem_values_are_values (| s2, r2 |) (snd #s1 #s2 fs_e) e2
 
-let fs_tail #t #g fsG =
-  on_dom
-    (x:var{Some? (g x)})
-    #(fun x -> get_Type (Some?.v (g x)))
-    (fun y -> fsG (y+1))
+let safety (t:qType) (fs_e:get_Type t) (e:closed_exp) : Lemma
+  (requires t ⦂ (fs_e, e))
+  (ensures safe e) =
+  introduce forall e'. steps e e' ==> is_value e' \/ can_step e' with begin
+    introduce steps e e' ==> is_value e' \/ can_step e' with _. begin
+      introduce irred e' ==> is_value e' with _. begin
+        assert (t ∋ (fs_e, e'));
+        lem_values_are_values t fs_e e';
+        assert (is_value e')
+      end
+    end
+  end
 
-let get_v #g fsG x = fsG x
+(** F* Evaluation Environment : variable -> value **)
 
-let lem_fs_stack_hd fsG v = ()
-let lem_fs_stack_get_v fsG v = ()
-let lem_fs_tail fsG = ()
+(** We compile F* values, not F* expressions.
+    When compiling F* lambdas, there is no way to match and get
+    the body of the lambda.
 
-let tail_stack_inverse #g fsG #t v =
-  let fsG' : fs_env g = fs_tail (fs_stack fsG v) in
-  assert (forall x. fsG' x == fsG x);
-  assert (feq fsG' fsG);
-  extensionality (x:var{Some? (g x)}) (fun x -> get_Type (Some?.v (g x))) fsG' fsG;
-  assert (fsG' == fsG)
+    To avoid this limitation, we do closure conversion of F* lambdas:
+    - be a lambda f:'a -> 'b
+    - we wrap f to a function that takes as argument an F* evaluation environment
+      that was extended to contain a value of type 'a
+    - we take the value from the environment to open f:
+        fun fsG -> f (index fsG 0)
+
+    What is cool about this is to define compilation to STLC the environment is abstract.
+ **)
+
+let (∽) (#g:typ_env) #b (fsG:eval_env g) (s:gsub g b) : Type0 =
+  forall (x:var). Some? (g x) ==>
+    Some?.v (g x) ∋ (index fsG x, s x)
+
+(** Cross Language Binary Logical Relation between F* and STLC expressions
+     for __open terms__. **)
+let equiv (#g:typ_env) (t:qType) (fs_e:fs_oexp g t) (e:exp) : Type0 =
+  fv_in_env g e /\
+  forall b (s:gsub g b) (fsG:eval_env g).
+    fsG ∽ s ==>  t ⦂ (fs_e fsG, gsubst s e)
+
+let (≈) (#g:typ_env) (#t:qType) (fs_v:fs_oexp g t) (e:exp) : Type0 =
+  equiv #g t fs_v e
+
+(** Equiv closed terms **)
+let equiv_closed_terms (#t:qType) (fs_e:get_Type t) (e:closed_exp) :
+  Lemma (requires equiv #empty t (fun _ -> fs_e) e)
+        (ensures  t ⦂ (fs_e, e)) =
+  eliminate forall b (s:gsub empty b) (fsG:eval_env empty).
+    fsG ∽ s ==>  t ⦂ ((fun _ -> fs_e) fsG, gsubst s e) with true gsub_empty empty_eval
+
+let lem_equiv_exp_are_equiv (g:typ_env) (#t:qType) (fs_e:get_Type t) (e:closed_exp) :
+  Lemma (requires t ⦂ (fs_e, e))
+        (ensures  equiv #empty t (fun _ -> fs_e) e) =
+  introduce forall b (s:gsub empty b) (fsG:eval_env empty).
+    fsG ∽ s ==>  t ⦂ ((fun _ -> fs_e) fsG, gsubst s e) with begin
+    assert (gsubst s e == e)
+  end
+
+(** Rules **)
+
+let tunit : qType =
+  (| _, QUnit |)
+
+let equiv_unit g
+  : Lemma ((fun (_:eval_env g) -> ()) `equiv tunit` EUnit)
+  = assert ((fun (_:eval_env g) -> ()) `equiv tunit` EUnit) by (explode ())
+
+let tbool : qType =
+  (| _, QBool |)
+
+let equiv_true g
+  : Lemma ((fun (_:eval_env g) -> true) `equiv tbool` ETrue)
+  = assert ((fun (_:eval_env g) -> true) `equiv tbool` ETrue) by (explode ())
+
+let equiv_false g
+  : Lemma ((fun (_:eval_env g) -> false) `equiv tbool` EFalse)
+  = assert ((fun (_:eval_env g) -> false) `equiv tbool` EFalse) by (explode ())
+
+let equiv_var g (x:var{Some? (g x)})
+  : Lemma ((fun (fsG:eval_env g) -> index fsG x) ≈ EVar x)
+  =
+  introduce forall b (s:gsub g b) fsG. fsG ∽ s ==>  Some?.v (g x) ⦂ (index fsG x, gsubst s (EVar x)) with begin
+    introduce _ ==> _ with _. begin
+      assert (Some?.v (g x) ∋ (index fsG x, s x));
+      lem_values_are_expressions (Some?.v (g x)) (index fsG x) (s x)
+    end
+  end
+
+let equiv_lam g (t1:qType) (t2:qType) (f:fs_oexp g (t1 ^-> t2)) (body:exp) : Lemma
+  (requires (fun (fsG:eval_env (extend t1 g)) -> f (tail #t1 fsG) (hd fsG)) ≈ body)
+  (ensures f ≈ (ELam body)) =
+  lem_fv_in_env_lam g t1 body;
+  let g' = extend t1 g in
+  introduce forall b (s:gsub g b) fsG. fsG ∽ s ==>  (t1 ^-> t2) ⦂ (f fsG, gsubst s (ELam body)) with begin
+    introduce _ ==> _ with _. begin
+      let body' = subst (sub_elam s) body in
+      assert (gsubst s (ELam body) == ELam body');
+      introduce forall (v:value) (fs_v:get_Type t1). t1 ∋ (fs_v, v) ==>  t2 ⦂ (f fsG fs_v, subst_beta v body') with begin
+        introduce _ ==> _ with _. begin
+          let s' = gsub_extend s t1 v in
+          let fsG' = stack fsG fs_v in
+          eliminate forall b (s':gsub g' b) (fsG':eval_env g'). fsG' ∽ s' ==>  t2 ⦂ (f (tail #t1 fsG') (hd #t1 #g fsG'), (gsubst s' body))
+            with false s' fsG';
+          assert (fsG ∽ s);
+          assert (stack fsG fs_v ∽ gsub_extend s t1 v);
+          assert (t2 ⦂ (f (tail fsG') (hd fsG'), (gsubst s' body)));
+          assert (hd (stack fsG fs_v) == fs_v);
+          assert (t2 ⦂ (f (tail fsG') fs_v, (gsubst s' body)));
+          assert (t2 ⦂ (f fsG fs_v, (gsubst s' body)));
+          lem_substitution s t1 v body;
+          assert (t2 ⦂ (f fsG fs_v, subst_beta v body'))
+        end
+      end;
+      assert ((t1 ^-> t2) ∋ (f fsG, gsubst s (ELam body)));
+      lem_values_are_expressions (t1 ^-> t2) (f fsG) (gsubst s (ELam body));
+      assert ((t1 ^-> t2) ⦂ (f fsG, gsubst s (ELam body)))
+    end
+  end
+
+let equiv_app g
+  (t1:qType) (t2:qType)
+  (fs_e1:fs_oexp g (t1 ^-> t2)) (fs_e2:fs_oexp g t1)
+  (e1:exp) (e2:exp)
+  : Lemma
+    (requires fs_e1 ≈ e1 /\ fs_e2 ≈ e2)
+    (ensures (fun fsG -> (fs_e1 fsG) (fs_e2 fsG)) ≈ (EApp e1 e2))
+  =
+  lem_fv_in_env_app g e1 e2;
+  introduce forall b (s:gsub g b) fsG. fsG ∽ s ==> t2 ⦂ ((fs_e1 fsG) (fs_e2 fsG), gsubst s (EApp e1 e2)) with begin
+    let fs_e1 = fs_e1 fsG in
+    let fs_e2 = fs_e2 fsG in
+    let fs_e = fs_e1 fs_e2 in
+    let e = EApp (gsubst s e1) (gsubst s e2) in
+    assert (gsubst s (EApp e1 e2) == e);
+    let EApp e1 e2 = e in
+    introduce fsG ∽ s ==>  t2 ⦂ (fs_e, e) with _. begin
+      introduce forall (e':closed_exp). steps e e' /\ irred e' ==> t2 ∋ (fs_e, e') with begin
+        introduce _ ==> t2 ∋ (fs_e, e') with h. begin
+          let steps_e_e' : squash (steps e e') = () in
+          FStar.Squash.map_squash #_ #(squash (t2 ∋ (fs_e, e'))) steps_e_e' (fun steps_e_e' ->
+            let (e11, e2') = destruct_steps_eapp e1 e2 e' steps_e_e' in
+            assert ((t1 ^-> t2) ∋ (fs_e1, ELam e11));
+            introduce True ==>  t1 ∋ (fs_e2, e2') with _. begin
+              assert (t1 ⦂ (fs_e2, e2));
+              assert (steps e2 e2');
+              assert (irred e2')
+            end;
+            eliminate forall (v:value) (fs_v:get_Type t1). t1 ∋ (fs_v, v) ==>
+              t2 ⦂ (fs_e1 fs_v, subst_beta v e11)
+            with e2' fs_e2;
+            assert (t2 ⦂ (fs_e, subst_beta e2' e11));
+            assert (t2 ∋ (fs_e, e'))
+          )
+        end
+      end
+    end
+  end
+
+let equiv_if g (t:qType) (fs_e1:fs_oexp g tbool) (fs_e2:fs_oexp g t) (fs_e3:fs_oexp g t) (e1:exp) (e2:exp) (e3:exp) : Lemma
+  (requires fs_e1 ≈ e1 /\ fs_e2 ≈ e2 /\ fs_e3 ≈ e3)
+  (ensures (fun fsG -> if fs_e1 fsG then fs_e2 fsG else fs_e3 fsG) ≈ EIf e1 e2 e3) =
+  lem_fv_in_env_if g e1 e2 e3;
+  introduce forall b (s:gsub g b) fsG. fsG ∽ s ==> t ⦂ ((if fs_e1 fsG then fs_e2 fsG else fs_e3 fsG), gsubst s (EIf e1 e2 e3)) with begin
+    let fs_e1 = fs_e1 fsG in
+    let fs_e = if fs_e1 then fs_e2 fsG else fs_e3 fsG in
+    let e = EIf (gsubst s e1) (gsubst s e2) (gsubst s e3) in
+    assert (gsubst s (EIf e1 e2 e3) == e);
+    let EIf e1 e2 e3 = e in
+    introduce fsG ∽ s ==>  t ⦂ (fs_e, e) with _. begin
+      introduce forall (e':closed_exp). steps e e' /\ irred e' ==> t ∋ (fs_e, e') with begin
+        introduce _ ==> t ∋ (fs_e, e') with h. begin
+          let steps_e_e' : squash (steps e e') = () in
+          FStar.Squash.map_squash #_ #(squash (t ∋ (fs_e, e'))) steps_e_e' (fun steps_e_e' ->
+            let e1' = destruct_steps_eif e1 e2 e3 e' steps_e_e' in
+            assert (tbool ∋ (fs_e1, e1'));
+            assert (t ∋ (fs_e, e'))
+          )
+        end
+      end
+    end
+  end
+
+let equiv_pair g (t1 t2:qType) (fs_e1:fs_oexp g t1) (fs_e2:fs_oexp g t2) (e1:exp) (e2:exp) : Lemma
+  (requires fs_e1 ≈ e1 /\ fs_e2 ≈ e2)
+  (ensures (fun fsG -> (fs_e1 fsG, fs_e2 fsG)) `equiv (t1 ^* t2)` EPair e1 e2) =
+  lem_fv_in_env_pair g e1 e2;
+  let t = t1 ^* t2 in
+  introduce forall b (s:gsub g b) fsG. fsG ∽ s ==>  t ⦂ ((fs_e1 fsG, fs_e2 fsG), gsubst s (EPair e1 e2)) with begin
+    let fs_e1 = fs_e1 fsG in
+    let fs_e2 = fs_e2 fsG in
+    let fs_e = (fs_e1, fs_e2) in
+    let e = EPair (gsubst s e1) (gsubst s e2) in
+    assert (gsubst s (EPair e1 e2) == e);
+    let EPair e1 e2 = e in
+    introduce fsG ∽ s ==>  t ⦂ (fs_e, e) with _. begin
+      introduce forall (e':closed_exp). steps e e' /\ irred e' ==> t ∋ (fs_e, e') with begin
+        introduce _ ==> t ∋ (fs_e, e') with h. begin
+          let steps_e_e' : squash (steps e e') = () in
+          FStar.Squash.map_squash #_ #(squash (t ∋ (fs_e, e'))) steps_e_e' (fun steps_e_e' ->
+            let (e1', e2') = destruct_steps_epair e1 e2 e' steps_e_e' in
+            assert (t1 ∋ (fs_e1, e1'));
+            assert (t2 ∋ (fs_e2, e2'));
+            assert (t ∋ (fs_e, EPair e1' e2'));
+            lem_values_are_expressions t fs_e (EPair e1' e2')
+          )
+        end
+      end
+    end
+  end
+
+let equiv_pair_fst_app g (t1 t2:qType) (fs_e12:fs_oexp g (t1 ^* t2)) (e12:exp) : Lemma
+  (requires fs_e12 `equiv (t1 ^* t2)` e12) (** is this too strict? we only care for the left to be equivalent. **)
+  (ensures (fun fsG -> fst (fs_e12 fsG)) `equiv t1` (EFst e12)) =
+  introduce forall b (s:gsub g b) fsG. fsG ∽ s ==>  t1 ⦂ (fst (fs_e12 fsG), gsubst s (EFst e12)) with begin
+    let fs_e12 = fs_e12 fsG in
+    let fs_e = fst fs_e12 in
+    let e = EFst (gsubst s e12) in
+    assert (gsubst s (EFst e12) == e);
+    let EFst e12 = e in
+    introduce fsG ∽ s ==>  t1 ⦂ (fs_e, e) with _. begin
+      introduce forall (e':closed_exp). steps e e' /\ irred e' ==> t1 ∋ (fs_e, e') with begin
+        introduce _ ==> t1 ∋ (fs_e, e') with h. begin
+          let steps_e_e' : squash (steps e e') = () in
+          FStar.Squash.map_squash #_ #(squash (t1 ∋ (fs_e, e'))) steps_e_e' (fun steps_e_e' ->
+            let e12' = destruct_steps_epair_fst e12 e' steps_e_e' in
+            eliminate (t1 ^* t2) ⦂ (fs_e12, e12) /\ steps e12 e12' /\ irred e12'
+            returns (t1 ^* t2) ∋ (fs_e12, e12') with _ _. ();
+            let EPair e1' e2' = e12' in
+            assert (t1 ∋ (fs_e, e1'));
+            lem_destruct_steps_epair_fst e1' e2' e';
+            assert (t1 ∋ (fs_e, e'))
+          )
+        end
+      end
+    end
+  end
+
+let equiv_pair_fst g (t1 t2:qType)
+  : Lemma
+    (requires True)
+    (ensures (fun _ -> fst #(get_Type t1) #(get_Type t2)) `equiv #g ((t1 ^* t2) ^-> t1)` (ELam (EFst (EVar 0))))
+  =
+  let tp = t1 ^* t2 in
+  let t = tp ^-> t1 in
+  let fs_e : (get_Type t1 & get_Type t2) -> get_Type t1 = fst in
+  let fs_e' : eval_env g -> get_Type t = (fun _ -> fs_e) in
+  let e = ELam (EFst (EVar 0)) in
+  introduce forall b (s:gsub g b) fsG. fsG ∽ s ==>  t ⦂ (fs_e' fsG, gsubst s e) with begin
+    assert (gsubst s e == e);
+    assert (fs_e' fsG == fs_e);
+
+    eliminate True /\ True
+    returns t ∋ (fs_e, e) with _ _. begin
+      introduce forall (v:value) (fs_v:get_Type tp). tp ∋ (fs_v, v) ==>
+        t1 ⦂ (fs_e fs_v, subst_beta v (EFst (EVar 0))) with begin
+        introduce _ ==> _ with _. begin
+          lem_values_are_expressions tp fs_v v;
+          lem_equiv_exp_are_equiv empty #tp fs_v v;
+          assert ((fun _ -> fs_v) `equiv #empty tp` v);
+          equiv_pair_fst_app empty t1 t2 (fun _ -> fs_v) v;
+          assert ((fun _ -> fs_e fs_v) `equiv #empty t1` (EFst v));
+          equiv_closed_terms #t1 (fs_e fs_v) (EFst v);
+          assert (subst_beta v (EFst (EVar 0)) == EFst v);
+          ()
+        end
+      end
+    end;
+
+    assert (t ∋ (fs_e, e));
+    lem_values_are_expressions t fs_e e;
+    assert (t ⦂ (fs_e, e))
+  end
+
+let equiv_pair_snd_app g (t1 t2:qType) (fs_e12:fs_oexp g (t1 ^* t2)) (e12:exp)
+  : Lemma
+    (requires fs_e12 `equiv (t1 ^* t2)` e12) (** is this too strict? we only care for the left to be equivalent. **)
+    (ensures (fun fsG -> snd (fs_e12 fsG)) `equiv t2` (ESnd e12))
+  =
+  introduce forall b (s:gsub g b) fsG. fsG ∽ s ==>  t2 ⦂ (snd (fs_e12 fsG), gsubst s (ESnd e12)) with begin
+    let fs_e12 = fs_e12 fsG in
+    let fs_e = snd fs_e12 in
+    let e = ESnd (gsubst s e12) in
+    assert (gsubst s (ESnd e12) == e);
+    let ESnd e12 = e in
+    introduce fsG ∽ s ==>  t2 ⦂ (fs_e, e) with _. begin
+      introduce forall (e':closed_exp). steps e e' /\ irred e' ==> t2 ∋ (fs_e, e') with begin
+        introduce _ ==> t2 ∋ (fs_e, e') with h. begin
+          let steps_e_e' : squash (steps e e') = () in
+          FStar.Squash.map_squash #_ #(squash (t2 ∋ (fs_e, e'))) steps_e_e' (fun steps_e_e' ->
+            let e12' = destruct_steps_epair_snd e12 e' steps_e_e' in
+            eliminate (t1 ^* t2) ⦂ (fs_e12, e12) /\ steps e12 e12' /\ irred e12'
+            returns (t1 ^* t2) ∋ (fs_e12, e12') with _ _. ();
+            let EPair e1' e2' = e12' in
+            assert (t2 ∋ (fs_e, e2'));
+            lem_destruct_steps_epair_snd e1' e2' e';
+            assert (t2 ∋ (fs_e, e'))
+          )
+        end
+      end
+    end
+  end
+
+let equiv_pair_snd g (t1 t2:qType)
+  : Lemma
+    (requires True)
+    (ensures (fun _ -> snd #(get_Type t1) #(get_Type t2)) `equiv #g ((t1 ^* t2) ^-> t2)` (ELam (ESnd (EVar 0))))
+  =
+  let tp = t1 ^* t2 in
+  let t = tp ^-> t2 in
+  let fs_e : (get_Type t1 & get_Type t2) -> get_Type t2 = snd in
+  let fs_e' : eval_env g -> get_Type t = (fun _ -> fs_e) in
+  let e = ELam (ESnd (EVar 0)) in
+  introduce forall b (s:gsub g b) fsG. fsG ∽ s ==>  t ⦂ (fs_e' fsG, gsubst s e) with begin
+    assert (gsubst s e == e);
+    assert (fs_e' fsG == fs_e);
+
+    eliminate True /\ True
+    returns t ∋ (fs_e, e) with _ _. begin
+      introduce forall (v:value) (fs_v:get_Type tp). tp ∋ (fs_v, v) ==>
+        t2 ⦂ (fs_e fs_v, subst_beta v (ESnd (EVar 0))) with begin
+        introduce _ ==> _ with _. begin
+          lem_values_are_expressions tp fs_v v;
+          lem_equiv_exp_are_equiv empty #tp fs_v v;
+          assert ((fun _ -> fs_v) `equiv #empty tp` v);
+          equiv_pair_snd_app empty t1 t2 (fun _ -> fs_v) v;
+          assert ((fun _ -> fs_e fs_v) `equiv #empty t2` (ESnd v));
+          equiv_closed_terms #t2 (fs_e fs_v) (ESnd v);
+          assert (subst_beta v (ESnd (EVar 0)) == ESnd v);
+          ()
+        end
+      end
+    end;
+
+    assert (t ∋ (fs_e, e));
+    lem_values_are_expressions t fs_e e;
+    assert (t ⦂ (fs_e, e))
+  end
