rupicola/stlc/QTyp.fst
@@ -1,158 +1,40 @@
 module QTyp
 
-open FStar.Tactics
-open FStar.Classical.Sugar
-open FStar.List.Tot
+open FStar.FunctionalExtensionality
 
-open STLC
+type eval_env g =
+  restricted_t (x:var{Some? (g x)}) (fun x -> get_Type (Some?.v (g x)))
 
-(** We define quotation for Type **)
+let empty_eval : eval_env empty =
+  on_dom
+    (x:var{Some? (empty x)})
+    #(fun x -> get_Type (Some?.v (empty x)))
+    (fun _ -> assert False)
 
-(** Cezar: why do we need quotation for types?
-      We use it to define the logical relation.
-**)
-noeq
-type type_quotation : Type0 -> Type u#1 =
-| QUnit : type_quotation unit
-| QBool : type_quotation bool
-| QArr : #s1:Type ->
-         #s2:Type ->
-         type_quotation s1 ->
-         type_quotation s2 ->
-         type_quotation (s1 -> s2)
-| QPair : #s1:Type ->
-          #s2:Type ->
-          type_quotation s1 ->
-          type_quotation s2 ->
-          type_quotation (s1 & s2)
+let hd #g fsG = fsG 0
 
-let (^->) #s1 #s2 = QArr #s1 #s2
-let (^*) #s1 #s2 = QPair #s1 #s2
+let stack #g fsG #t fs_v =
+  on_dom
+    (x:var{Some? ((extend t g) x)})
+    #(fun x -> get_Type (Some?.v ((extend t g) x)))
+    (fun y ->
+      if y = 0 then fs_v else fsG (y-1))
 
-let test_match s (r:type_quotation s) = (** why does this work so well? **)
-  match r with
-  | QUnit -> assert (s == unit)
-  | QBool -> assert (s == bool)
-  | QArr #s1 #s2 _ _ -> assert (s == (s1 -> s2))
-  | QPair #s1 #s2 _ _ -> assert (s == (s1 & s2))
+let tail #t #g fsG =
+  on_dom
+    (x:var{Some? (g x)})
+    #(fun x -> get_Type (Some?.v (g x)))
+    (fun y -> fsG (y+1))
 
-let rec type_quotation_to_typ s (r:type_quotation s) : typ =
-  match r with
-  | QUnit -> TUnit
-  | QBool -> TBool
-  | QArr #s1 #s2 rs1 rs2 -> TArr (type_quotation_to_typ s1 rs1) (type_quotation_to_typ s2 rs2)
-  | QPair #s1 #s2 rs1 rs2 -> TPair (type_quotation_to_typ s1 rs1) (type_quotation_to_typ s2 rs2)
+let index #g fsG x = fsG x
 
-(** Type of Quotable Types **)
-type qType =
-  s:Type & type_quotation s
+let lem_stack_hd fsG v = ()
+let lem_stack_index fsG v = ()
+let lem_index_tail fsG = ()
 
-let get_Type (t:qType) = t._1
-let get_rel (t:qType) = t._2
-
-let mk_arrow (t1 t2:qType) : qType =
-  (| _, (get_rel t1) ^-> (get_rel t2) |)
-
-let mk_pair (t1 t2:qType) : qType =
-  (| _, (get_rel t1) ^* (get_rel t2) |)
-
-(** typ_env is a typing environment: variables to Quotable Types **)
-type env = var -> option qType
-let empty : env = fun _ -> None
-
-(* we only need extend at 0 *)
-let extend (t:qType) (g:env)
-  : env
-  = fun y -> if y = 0 then Some t
-          else g (y-1)
-
-let fv_in_env (g:env) (e:exp) : Type0 =
-  forall (fv:var). fv `memP` free_vars e ==> Some? (g fv)
-
-let lem_no_fv_is_closed (e:exp) : Lemma
-  (requires fv_in_env empty e)
-  (ensures is_closed e)
-  [SMTPat (is_closed e)] =
-  ()
-
-let lem_closed_is_no_fv (e:exp) : Lemma
-  (requires is_closed e)
-  (ensures fv_in_env empty e)
-  [SMTPat (is_closed e)] =
-  ()
-
-let lem_fv_in_env_lam (g:env) (t:qType) (body:exp) :
-  Lemma
-    (requires fv_in_env (extend t g) body)
-    (ensures  fv_in_env g (ELam body)) = admit ()
-
-let lem_fv_in_env_app (g:env) (e1 e2:exp) :
-  Lemma
-    (requires fv_in_env g e1 /\ fv_in_env g e2)
-    (ensures  fv_in_env g (EApp e1 e2)) = admit ()
-
-let lem_app_fv_in_env (g:env) (e1 e2:exp) :
-  Lemma
-    (requires fv_in_env g (EApp e1 e2))
-    (ensures fv_in_env g e1 /\ fv_in_env g e2) = admit ()
-
-let lem_fv_in_env_if (g:env) (e1 e2 e3:exp) :
-  Lemma
-    (requires fv_in_env g e1 /\ fv_in_env g e2 /\ fv_in_env g e3)
-    (ensures  fv_in_env g (EIf e1 e2 e3)) = admit ()
-
-let lem_if_fv_in_env (g:env) (e1 e2 e3:exp) :
-  Lemma
-    (requires fv_in_env g (EIf e1 e2 e3))
-    (ensures fv_in_env g e1 /\ fv_in_env g e2 /\ fv_in_env g e3) = admit ()
-
-let lem_fv_in_env_pair (g:env) (e1 e2:exp) :
-  Lemma
-    (requires fv_in_env g e1 /\ fv_in_env g e2)
-    (ensures  fv_in_env g (EPair e1 e2)) = admit ()
-
-let lem_pair_fv_in_env (g:env) (e1 e2:exp) :
-  Lemma
-    (requires fv_in_env g (EPair e1 e2))
-    (ensures fv_in_env g e1 /\ fv_in_env g e2) = admit ()
-
-let lem_fst_fv_in_env (g:env) (e:exp) : // this only makes sense because of how we defined free_vars_indx
-  Lemma
-    (requires fv_in_env g (EFst e))
-    (ensures fv_in_env g e) = admit ()
-
-let lem_snd_fv_in_env (g:env) (e:exp) :
-  Lemma
-    (requires fv_in_env g (ESnd e))
-    (ensures fv_in_env g e) = admit ()
-
-let lem_lam_fv_in_env (g:env) (body:exp) (t1:qType) :
-  Lemma
-    (requires fv_in_env g (ELam body))
-    (ensures fv_in_env (extend t1 g) body) = admit ()
-
-(** STLC Evaluation Environment : variable -> value **)
-let gsub (g:env) (b:bool{b ==> (forall x. None? (g x))}) = (** CA: this b is polluting **)
-  s:(sub b){forall x. Some? (g x) ==> is_value (s x)}
-
-let gsub_empty : gsub empty true =
-  (fun v -> EVar v)
-
-let gsub_extend (#g:env) #b (s:gsub g b) (t:qType) (v:value) : gsub (extend t g) false =
-  let f = fun (y:var) -> if y = 0 then v else s (y-1) in
-  introduce exists (x:var). ~(EVar? (f x)) with 0 and ();
-  f
-
-let gsubst (#g:env) #b (s:gsub g b) (e:exp{fv_in_env g e}) : closed_exp =
-  lem_subst_freevars_closes_exp s e 0;
-  subst s e
-
-let lem_substitution #g #b (s:gsub g b) (t:qType) (v:value) (e:exp)
-  : Lemma (
-    (subst (sub_beta v) (subst (sub_elam s) e)) == (subst (gsub_extend s t v) e))
-  = admit () (** common lemma **)
-
-let lem_gsubst_closed_identiy #g #b (s:gsub g b) (e:closed_exp) :
-  Lemma (gsubst s e == e)
-  [SMTPat (gsubst s e)] =
-  admit ()
+let tail_stack_inverse #g fsG #t v =
+  let fsG' : eval_env g = tail (stack fsG v) in
+  assert (forall x. fsG' x == fsG x);
+  assert (feq fsG' fsG);
+  extensionality (x:var{Some? (g x)}) (fun x -> get_Type (Some?.v (g x))) fsG' fsG;
+  assert (fsG' == fsG)
